VCVio.lean
@@ -1,7 +1,8 @@
 import VCVio.CryptoFoundations.AKE.Game
+import VCVio.CryptoFoundations.AKE.ICCA.Basic
+import VCVio.CryptoFoundations.AKE.ICCA.OfAsymmEncAlg
 import VCVio.CryptoFoundations.AKE.Interactive.Protocol
 import VCVio.CryptoFoundations.AKE.UAKE
-import VCVio.CryptoFoundations.AKE.iCCA
 import VCVio.CryptoFoundations.AKE.iCMA
 import VCVio.CryptoFoundations.AsymmEncAlg.Defs
 import VCVio.CryptoFoundations.AsymmEncAlg.INDCCA
